base code

BoilerPlate/Ex2.dfy
@@ -1,3 +1,8 @@
+function sorted(s : seq<int>) : bool {
+  forall k1, k2 :: 0 <= k1 <= k2 < |s| ==> s[k1] <= s[k2]
+}
+
+
 // Ex1
 method copy(a : array<int>, l : int, r : int) returns (ret : array<int>)
   requires 0 <= l < r <= a.Length 
@@ -12,8 +17,36 @@ method copy(a : array<int>, l : int, r : int) returns (ret : array<int>)
     invariant forall k :: 0 <= k < i ==> ret[k] == a[l + k] // 'ret' should contain copied elements
     decreases len - i 
   {
-
+    
     ret[i] := a[l + i]; // Copy the element from 'a' to 'ret' at the current index.
     i := i + 1;
   }
 }
+
+
+// Ex2
+
+method mergeArr(a : array<int>, l : int, m : int, r : int) 
+  requires 0 <= l < m < r <= a.Length  
+  requires sorted(a[l..m]) && sorted(a[m..r])
+  ensures sorted(a[l..r]) 
+  ensures a[..l] == old(a[..l])
+  ensures a[r..] == old(a[r..]) 
+  modifies a 
+{
+ // ToDo 
+}
+
+
+// Ex3
+method sort (a : array<int>) 
+  ensures sorted(a[..])
+  modifies a 
+{
+  // ToDo
+}
+
+
+
+
+
