BoilerPlate/Ex1.dfy
@@ -1,0 +1,39 @@
+datatype Tree<V> = Leaf(V) | SingleNode(V, Tree<V>) | DoubleNode(V, Tree<V>, Tree<V>)
+
+datatype Code<V> = CLf(V) | CSNd(V) | CDNd(V)
+
+function serialise<V>(t : Tree<V>) : seq<Code<V>> 
+  decreases t 
+{
+  match t {
+    case Leaf(v) => [ CLf(v) ]
+    case SingleNode(v, t) => serialise(t) + [ CSNd(v) ]
+    case DoubleNode(v, t1, t2) => serialise(t2) + serialise(t1) + [ CDNd(v) ]
+  }
+}
+
+
+// Ex 1
+function deserialise<V>(cs : seq<Code<V>>) : Tree<V> 
+{
+  // ToDo
+}
+
+
+// Ex 2
+
+
+// Ex 3 
+
+// Ex 4 
+
+lemma SerialiseLemma<V>(t : Tree<V>)
+  ensures deserialise(serialise(t)) == t 
+{
+  // ToDo
+}
+
+
+
+
+
