BoilerPlate/Ex3.dfy
@@ -1,0 +1,79 @@
+
+module Ex3 {
+
+
+class Node {
+
+  var data : int 
+  var next : Node? 
+
+  ghost var list : seq<int>
+  ghost var footprint : set<Node>
+
+  ghost function Valid() : bool 
+    reads this, footprint
+    decreases footprint
+  {
+    (this in footprint) &&
+    ((next == null) ==> list == [ data ] && footprint == { this }) &&
+    ((next != null) ==> 
+      (next in footprint) && 
+      footprint == next.footprint + { this } && 
+      (this !in next.footprint) &&
+      list == [ data ] + next.list &&
+      next.Valid())
+  }
+
+  constructor (val : int) 
+    ensures Valid() 
+      && next == null && list == [ data ] 
+      && footprint == { this } 
+      && val == data 
+  {
+    this.data := val; 
+    this.next := null; 
+    this.list := [ val ]; 
+    this.footprint := { this };
+  } 
+
+  method prepend (val : int) returns (r : Node)
+    requires Valid()
+    ensures r.Valid()
+    ensures r.list == [ val ] + this.list
+    ensures r.footprint == { r } + this.footprint
+    ensures fresh(r) 
+  {
+    r := new Node(val); 
+    r.next := this; 
+    r.footprint := { r } + this.footprint; 
+    r.list := [ val ] + this.list;  
+    return; 
+  }
+
+
+  // Ex1
+  method reverse(tail : Node?) returns (r : Node) 
+  {
+    var old_next := this.next; 
+    this.next := tail; 
+    
+    if (old_next == null) {
+      r := this; 
+      return; 
+    } else {
+      r := old_next.reverse(this);
+      return;  
+    }
+  }
+
+}
+
+
+// Ex2
+
+method ExtendList(lst : Node?, v : int) returns (r : Node) 
+{
+  // ToDo 
+}
+
+}
