BoilerPlate/Ex4.dfy
@@ -1,0 +1,49 @@
+include "Ex3.dfy"
+
+
+module Ex4 {
+
+
+import Ex3=Ex3
+
+class Queue {
+
+  var lst1 : Ex3.Node?
+  var lst2 : Ex3.Node? 
+
+  // Ex1
+  ghost function Valid() : bool 
+  {
+    // ToDo  
+  }
+
+  // Ex2 
+  constructor () 
+  {
+    this.lst1 := null; 
+    this.lst2 := null;  
+    // ToDo
+  } 
+
+  // Ex3.1
+  method push(val : int) 
+  {
+    lst1 := Ex3.ExtendList(lst1, val);     
+  }
+
+  // Ex3.2
+  method pop() returns (r : int)
+  {
+
+    if (lst2 == null) {
+      lst2 := lst1.reverse(null); 
+      lst1 := null;
+    }
+
+    r := lst2.data; 
+    lst2 := lst2.next; 
+  }
+  
+}
+
+}
